some refactoring of the soundness module

pulse/examples/dsls/mini_steel/Pulse.Soundness.Exists.fst
@@ -1,6 +1,158 @@
 module Pulse.Soundness.Exists
 
-let exists_inversion _ = admit ()
-let elim_exists_soundness _ _ _ = admit ()
-let intro_exists_soundness _ _ _ = admit ()
-let intro_exists_erased_soundness _ _ _ = admit ()
+module R = FStar.Reflection
+module RT = Refl.Typing
+
+open Pulse.Syntax
+open Pulse.Reflection.Util
+open Pulse.Typing
+open Pulse.Elaborate.Pure
+open Pulse.Elaborate.Core
+open Pulse.Elaborate
+open Pulse.Soundness.Common
+
+module WT = Pulse.Steel.Wrapper.Typing
+module LN = Pulse.Typing.LN
+module FV = Pulse.Typing.FV
+
+#push-options "--fuel 4 --ifuel 1"
+let intro_exists_erased_soundness
+  (#f:stt_env)
+  (#g:env)
+  (#t:st_term)
+  (#c:comp)
+  (d:st_typing f g t c{T_IntroExistsErased? d})
+  : GTot (RT.typing (extend_env_l f g)
+                    (elab_st_typing d)
+                    (elab_comp c)) =
+  let t0 = t in
+  let T_IntroExistsErased _ u t p e t_typing p_typing e_typing = d in
+  let ru = elab_universe u in
+  let rt = elab_term t in
+  let rp = elab_term p in
+  let re = elab_term e in
+  let rt_typing : RT.typing _ rt (R.pack_ln (R.Tv_Type ru)) =
+      tot_typing_soundness t_typing in
+
+  let rp_typing
+      : RT.typing _
+                  (mk_exists ru rt (mk_abs rt R.Q_Explicit rp)) vprop_tm =
+      tot_typing_soundness p_typing
+  in
+  let rp_typing
+      : RT.typing _
+                  (mk_abs rt R.Q_Explicit rp)
+                  (mk_arrow (rt, R.Q_Explicit) vprop_tm) =
+        WT.exists_inversion rp_typing
+  in
+  let re_typing : RT.typing _ re _ =
+      tot_typing_soundness e_typing
+  in
+  let reveal_re = elab_term (mk_reveal u t e) in
+
+  // reveal_re is ln
+  LN.tot_typing_ln e_typing;
+  elab_ln (mk_reveal u t e) (-1);
+
+  //rp is (ln' 0)
+  LN.tot_typing_ln p_typing;
+  elab_ln p 0;
+  
+  RT.beta_reduction rt R.Q_Explicit rp reveal_re;    
+
+  WT.intro_exists_erased_typing rt_typing rp_typing re_typing
+
+let intro_exists_soundness
+  (#f:stt_env)
+  (#g:env)
+  (#t:st_term)
+  (#c:comp)
+  (d:st_typing f g t c{T_IntroExists? d })
+  : GTot (RT.typing (extend_env_l f g)
+                    (elab_st_typing d)
+                    (elab_comp c)) =
+
+  let t0 = t in
+  let T_IntroExists _ u t p e t_typing p_typing e_typing = d in
+  let ru = elab_universe u in
+  let rt = elab_term t in
+  let rp = elab_term p in
+  let re = elab_term e in
+  let rt_typing : RT.typing _ rt (R.pack_ln (R.Tv_Type ru)) =
+      tot_typing_soundness t_typing in
+  let rp_typing
+      : RT.typing _
+                  (mk_exists ru rt (mk_abs rt R.Q_Explicit rp)) vprop_tm =
+      tot_typing_soundness p_typing in
+  let rp_typing
+      : RT.typing _
+                  (mk_abs rt R.Q_Explicit rp)
+                  (mk_arrow (rt, R.Q_Explicit) vprop_tm) =
+        WT.exists_inversion rp_typing
+  in
+  let re_typing : RT.typing _ re _ =
+      tot_typing_soundness e_typing
+  in
+
+  // re is ln
+  LN.tot_typing_ln e_typing;
+  elab_ln e (-1);
+
+  //rp is (ln' 0)
+  LN.tot_typing_ln p_typing;
+  elab_ln p 0;
+
+  RT.beta_reduction rt R.Q_Explicit rp re;
+
+  WT.intro_exists_typing rt_typing rp_typing re_typing
+#pop-options
+
+#push-options "--z3rlimit_factor 8 --fuel 4 --ifuel 2"
+let elim_exists_soundness
+  (#f:stt_env)
+  (#g:env)
+  (#t:st_term)
+  (#c:comp)
+  (d:st_typing f g t c{T_ElimExists? d})
+  : GTot (RT.typing (extend_env_l f g)
+                    (elab_st_typing d)
+                    (elab_comp c)) =
+
+  let T_ElimExists _ u t p x t_typing p_typing = d in
+  let ru = elab_universe u in
+  let rt = elab_term t in
+  let rp = elab_term p in
+  let rt_typing = tot_typing_soundness t_typing in
+  let rp_typing
+    : RT.typing (extend_env_l f g)
+                (mk_exists ru (elab_term t)
+                   (mk_abs (elab_term t) R.Q_Explicit (elab_term p)))
+                vprop_tm
+    = tot_typing_soundness p_typing in
+  let rp_typing = WT.exists_inversion rp_typing in
+
+  FV.st_typing_freevars_inv d x;
+  assert (~ (Set.mem x (freevars t)));
+  assert (~ (Set.mem x (freevars p)));
+
+  let x_tm = Tm_Var {nm_index=x;nm_ppname=RT.pp_name_default} in
+  let rx_tm = R.pack_ln (R.Tv_Var (R.pack_bv (RT.make_bv x tun))) in
+  let rx_bv = R.pack_ln (R.Tv_BVar (R.pack_bv (RT.make_bv 0 tun))) in
+
+  // rt is ln
+  LN.tot_typing_ln t_typing;
+  elab_ln t (-1);
+
+  //rp is (ln' 0)
+  LN.tot_typing_ln p_typing;
+  elab_ln p 0;
+
+  calc (==) {
+    elab_term (close_term' (open_term' p (mk_reveal u t x_tm) 0) x 0);
+       (==) {
+               RT.beta_reduction rt R.Q_Explicit rp (Pulse.Reflection.Util.mk_reveal ru rt rx_tm)
+            }
+    WT.elim_exists_post_body ru rt (mk_abs rt R.Q_Explicit rp) x;
+  };
+  WT.elim_exists_typing x rt_typing rp_typing
+#pop-options
