pulse/examples/dsls/mini_steel/Pulse.Soundness.Par.fst
@@ -1,3 +1,103 @@
 module Pulse.Soundness.Par
 
-let par_soundness _ _ _ _ _ _ _ _ _ = admit ()
+open Pulse.Syntax
+open Pulse.Reflection.Util
+open Pulse.Typing
+open Pulse.Elaborate.Pure
+open Pulse.Elaborate.Core
+open Pulse.Elaborate
+open Pulse.Soundness.Common
+
+module R = FStar.Reflection
+
+module WT = Pulse.Steel.Wrapper.Typing
+
+
+#push-options "--z3rlimit_factor 10 --fuel 8 --ifuel 1"
+let par_soundness
+  (#f:stt_env)
+  (#g:env)
+  (#t:st_term)
+  (#c:comp)
+  (d:st_typing f g t c{T_Par? d})
+  (soundness: soundness_t d)
+  : GTot (RT.typing (extend_env_l f g)
+                    (elab_st_typing d)
+                    (elab_comp c)) =
+
+  let T_Par _ eL cL eR cR x cL_typing cR_typing eL_typing eR_typing = d in
+
+  let ru = elab_universe (comp_u cL) in
+  let raL = elab_term (comp_res cL) in
+  let raR = elab_term (comp_res cR) in
+  let rpreL = elab_term (comp_pre cL) in
+  let rpostL = mk_abs raL R.Q_Explicit (elab_term (comp_post cL)) in
+  let rpreR = elab_term (comp_pre cR) in
+  let rpostR = mk_abs raR R.Q_Explicit (elab_term (comp_post cR)) in
+  let reL = elab_st_typing eL_typing in
+  let reR = elab_st_typing eR_typing in
+
+  let reL_typing
+    : RT.typing _ reL (elab_comp cL) =
+    soundness f g eL cL eL_typing in
+
+  let reR_typing
+    : RT.typing _ reR (elab_comp cR) =
+    soundness f g eR cR eR_typing in
+
+  let (raL_typing, rpreL_typing, rpostL_typing)
+    : (RT.typing _ raL (R.pack_ln (R.Tv_Type ru)) &
+       RT.typing _ rpreL vprop_tm &
+       RT.typing _ rpostL (mk_arrow (raL, R.Q_Explicit) vprop_tm)) =
+
+    inversion_of_stt_typing f g cL ru (Comp.comp_typing_soundness f g cL (comp_u cL) cL_typing) in
+
+  let (raR_typing, rpreR_typing, rpostR_typing)
+    : (RT.typing _ raR (R.pack_ln (R.Tv_Type ru)) &
+       RT.typing _ rpreR vprop_tm &
+       RT.typing _ rpostR (mk_arrow (raR, R.Q_Explicit) vprop_tm)) =
+
+    inversion_of_stt_typing f g cR ru (Comp.comp_typing_soundness f g cR (comp_u cR) cR_typing) in
+
+  /////
+  let uL = comp_u cL in
+  let uR = comp_u cR in
+  let aL = comp_res cL in
+  let aR = comp_res cR in
+  let postL = comp_post cL in
+  let postR = comp_post cR in
+  let x_tm = term_of_var x in
+
+  // ln proofs for invoking the RT beta reduction
+  RT.well_typed_terms_are_ln _ _ _ raL_typing;
+  RT.well_typed_terms_are_ln _ _ _ raR_typing;
+  RT.well_typed_terms_are_ln _ _ _ rpostL_typing;
+  RT.well_typed_terms_are_ln _ _ _ rpostR_typing;
+
+  calc (==) {
+    elab_term (par_post uL uR aL aR postL postR x);
+       (==) { }
+    RT.open_or_close_term'
+      (mk_star
+         (RT.open_or_close_term'
+            (elab_term postL)
+            (RT.OpenWith (elab_term (mk_fst uL uR aL aR x_tm))) 0)
+         (RT.open_or_close_term'
+            (elab_term postR)
+            (RT.OpenWith (elab_term (mk_snd uL uR aL aR x_tm))) 0))
+      (RT.CloseVar x)
+      0;
+       (==) { RT.beta_reduction raL R.Q_Explicit
+                (elab_term postL)
+                (Pulse.Reflection.Util.mk_fst ru ru raL raR (RT.var_as_term x));
+              RT.beta_reduction raR R.Q_Explicit
+                (elab_term postR)
+                (Pulse.Reflection.Util.mk_snd ru ru raL raR (RT.var_as_term x)) }
+    WT.par_post ru raL raR rpostL rpostR x;
+  };
+  /////
+
+  WT.par_typing x raL_typing raR_typing rpreL_typing rpostL_typing
+    rpreR_typing rpostR_typing
+    reL_typing reR_typing
+#pop-options
