pulse/examples/dsls/mini_steel/Pulse.Soundness.Return.fst
@@ -1,12 +1,66 @@
 module Pulse.Soundness.Return
 
-open FStar.Reflection
-open Refl.Typing
-module RT = Refl.Typing
+open Pulse.Syntax
+open Pulse.Reflection.Util
+open Pulse.Typing
+open Pulse.Elaborate.Pure
+open Pulse.Elaborate.Core
+open Pulse.Elaborate
+open Pulse.Soundness.Common
 
-let return_stt_typing _ _ _ = admit ()
-let return_stt_noeq_typing _ _ _ = admit ()
-let return_stt_atomic_typing _ _ _ = admit ()
-let return_stt_atomic_noeq_typing _ _ _ = admit ()
-let return_stt_ghost_typing _ _ _ = admit ()
-let return_stt_ghost_noeq_typing _ _ _ = admit ()
+module R = FStar.Reflection
+
+module WT = Pulse.Steel.Wrapper.Typing
+module LN = Pulse.Typing.LN
+
+#push-options "--z3rlimit_factor 10 --fuel 4 --ifuel 2"
+let return_soundess
+  (#f:stt_env)
+  (#g:env)
+  (#t:st_term)
+  (#c:comp)
+  (d:st_typing f g t c{T_Return? d})
+  : GTot (RT.typing (extend_env_l f g)
+                    (elab_st_typing d)
+                    (elab_comp c)) =
+
+  let T_Return _ ctag use_eq u t e post x t_typing e_typing post_typing = d in
+  let ru = elab_universe u in
+  let rt = elab_term t in
+  let re = elab_term e in
+  let rpost = elab_term post in
+  let rpost = mk_abs rt R.Q_Explicit rpost in
+  let rt_typing : RT.typing _ rt (R.pack_ln (R.Tv_Type ru)) =
+    tot_typing_soundness t_typing in
+  let re_typing : RT.typing _ re rt =
+    tot_typing_soundness e_typing in
+  let rpost_typing
+    : RT.typing _ rpost
+                  (mk_arrow (rt, R.Q_Explicit) vprop_tm) =
+    mk_t_abs_tot f g RT.pp_name_default t_typing post_typing in
+
+  // re is ln
+  LN.tot_typing_ln e_typing;
+  elab_ln e (-1);
+
+  // (elab_term post) is (ln 0)
+  RT.well_typed_terms_are_ln _ rpost _ rpost_typing;
+  assert (RT.ln' (elab_term post) 0);
+
+  elab_open_commute' post e 0;
+  RT.beta_reduction rt R.Q_Explicit (elab_term post) re;
+  
+  match ctag, use_eq with
+  | STT, true ->
+    WT.return_stt_typing x rt_typing re_typing rpost_typing
+  | STT, false -> 
+    WT.return_stt_noeq_typing rt_typing re_typing rpost_typing
+  | STT_Atomic, true ->
+    WT.return_stt_atomic_typing x rt_typing re_typing rpost_typing
+  | STT_Atomic, false -> 
+    WT.return_stt_atomic_noeq_typing rt_typing re_typing rpost_typing
+  | STT_Ghost, true ->
+    WT.return_stt_ghost_typing x rt_typing re_typing rpost_typing
+  | STT_Ghost, false -> 
+    WT.return_stt_ghost_noeq_typing rt_typing re_typing rpost_typing
+#pop-options
