pulse/examples/dsls/mini_steel/Pulse.Soundness.Return.fsti
@@ -1,113 +1,19 @@
 module Pulse.Soundness.Return
 
-open FStar.Reflection
-open Pulse.Reflection.Util
+open Pulse.Syntax
+open Pulse.Typing
+open Pulse.Elaborate.Pure
+open Pulse.Elaborate.Core
+open Pulse.Soundness.Common
 
 module RT = Refl.Typing
 
-let return_post_with_eq (u:universe) (a:term) (e:term) (p:term) (x:var) : term =
-  let x_tm = RT.var_as_term x in
-  let eq2_tm =
-    let t = pack_ln (Tv_UInst (pack_fv (mk_steel_wrapper_lid "eq2_prop")) [u]) in
-    let t = pack_ln (Tv_App t (a, Q_Implicit)) in
-    let t = pack_ln (Tv_App t (x_tm, Q_Explicit)) in
-    pack_ln (Tv_App t (e, Q_Explicit)) in
-
-  let p_app_x = pack_ln (Tv_App p (x_tm, Q_Explicit)) in
-  
-  let star_tm = mk_star p_app_x eq2_tm in
-
-  mk_abs a Q_Explicit (RT.open_or_close_term' star_tm (RT.CloseVar x) 0)
-
-val return_stt_typing
+val return_soundess
+  (#f:stt_env)
   (#g:env)
-  (#u:universe)
-  (#a:term)
-  (#e:term)
-  (#p:term)
-  (x:var{None? (RT.lookup_bvar g x)})
-  (a_typing:RT.typing g a (pack_ln (Tv_Type u)))
-  (e_typing:RT.typing g e a)
-  (p_typing:RT.typing g p (mk_arrow (a, Q_Explicit) vprop_tm))
-
-  : GTot (RT.typing g
-                    (mk_stt_return u a e p)
-                    (mk_stt_comp u a
-                       (pack_ln (Tv_App p (e, Q_Explicit)))
-                       (return_post_with_eq u a e p x)))
-
-val return_stt_noeq_typing
-  (#g:env)
-  (#u:universe)
-  (#a:term)
-  (#x:term)
-  (#p:term)
-  (a_typing:RT.typing g a (pack_ln (Tv_Type u)))
-  (x_typing:RT.typing g x a)
-  (p_typing:RT.typing g p (mk_arrow (a, Q_Explicit) vprop_tm))
-
-  : GTot (RT.typing g
-                    (mk_stt_return u a x p)
-                    (mk_stt_comp u a (pack_ln (Tv_App p (x, Q_Explicit))) p))
-
-val return_stt_atomic_typing
-  (#g:env)
-  (#u:universe)
-  (#a:term)
-  (#e:term)
-  (#p:term)
-  (x:var{None? (RT.lookup_bvar g x)})
-  (a_typing:RT.typing g a (pack_ln (Tv_Type u)))
-  (e_typing:RT.typing g e a)
-  (p_typing:RT.typing g p (mk_arrow (a, Q_Explicit) vprop_tm))
-
-  : GTot (RT.typing g
-                    (mk_stt_atomic_return u a e p)
-                    (mk_stt_atomic_comp u a emp_inames_tm
-                       (pack_ln (Tv_App p (e, Q_Explicit)))
-                       (return_post_with_eq u a e p x)))
-
-val return_stt_atomic_noeq_typing
-  (#g:env)
-  (#u:universe)
-  (#a:term)
-  (#x:term)
-  (#p:term)
-  (a_typing:RT.typing g a (pack_ln (Tv_Type u)))
-  (x_typing:RT.typing g x a)
-  (p_typing:RT.typing g p (mk_arrow (a, Q_Explicit) vprop_tm))
-
-  : GTot (RT.typing g
-                    (mk_stt_atomic_return_noeq u a x p)
-                    (mk_stt_atomic_comp u a emp_inames_tm (pack_ln (Tv_App p (x, Q_Explicit))) p))
-
-val return_stt_ghost_typing
-  (#g:env)
-  (#u:universe)
-  (#a:term)
-  (#e:term)
-  (#p:term)
-  (x:var{None? (RT.lookup_bvar g x)})
-  (a_typing:RT.typing g a (pack_ln (Tv_Type u)))
-  (e_typing:RT.typing g e a)
-  (p_typing:RT.typing g p (mk_arrow (a, Q_Explicit) vprop_tm))
-
-  : GTot (RT.typing g
-                    (mk_stt_ghost_return u a e p)
-                    (mk_stt_ghost_comp u a emp_inames_tm
-                       (pack_ln (Tv_App p (e, Q_Explicit)))
-                       (return_post_with_eq u a e p x)))
-
-val return_stt_ghost_noeq_typing
-  (#g:env)
-  (#u:universe)
-  (#a:term)
-  (#x:term)
-  (#p:term)
-  (a_typing:RT.typing g a (pack_ln (Tv_Type u)))
-  (x_typing:RT.typing g x a)
-  (p_typing:RT.typing g p (mk_arrow (a, Q_Explicit) vprop_tm))
-
-  : GTot (RT.typing g
-                    (mk_stt_ghost_return_noeq u a x p)
-                    (mk_stt_ghost_comp u a emp_inames_tm (pack_ln (Tv_App p (x, Q_Explicit))) p))
+  (#t:st_term)
+  (#c:comp)
+  (d:st_typing f g t c{T_Return? d})
+  : GTot (RT.typing (extend_env_l f g)
+                    (elab_st_typing d)
+                    (elab_comp c))
