pulse/examples/dsls/mini_steel/Pulse.Soundness.Admit.fsti
@@ -1,59 +1,19 @@
 module Pulse.Soundness.Admit
 
-open FStar.Reflection
-open Pulse.Reflection.Util
+open Pulse.Syntax
+open Pulse.Typing
+open Pulse.Elaborate.Pure
+open Pulse.Elaborate.Core
+open Pulse.Soundness.Common
 
 module RT = Refl.Typing
 
-
-(*
-
- g |- a : Type u
- g |- p : vprop
- g |- q : a -> vprop
- ------------------------------------------
- g |- stt_admit a p q : stt a p q
-
-*)
-
-val stt_admit_soundness
+val admit_soundess
+  (#f:stt_env)
   (#g:env)
-  (#u:universe)
-  (#a:term)
-  (#p:term)
-  (#q:term)
-  (a_typing:RT.typing g a (pack_ln (Tv_Type u)))
-  (p_typing:RT.typing g p vprop_tm)
-  (q_typing:RT.typing g q (mk_arrow (a, Q_Explicit) vprop_tm))
-
-  : GTot (RT.typing g
-                    (mk_stt_admit u a p q)
-                    (mk_stt_comp u a p q))
-               
-val stt_atomic_admit_soundness
-  (#g:env)
-  (#u:universe)
-  (#a:term)
-  (#p:term)
-  (#q:term)
-  (a_typing:RT.typing g a (pack_ln (Tv_Type u)))
-  (p_typing:RT.typing g p vprop_tm)
-  (q_typing:RT.typing g q (mk_arrow (a, Q_Explicit) vprop_tm))
-
-  : GTot (RT.typing g
-                    (mk_stt_atomic_admit u a p q)
-                    (mk_stt_atomic_comp u a emp_inames_tm p q))
-
-val stt_ghost_admit_soundness
-  (#g:env)
-  (#u:universe)
-  (#a:term)
-  (#p:term)
-  (#q:term)
-  (a_typing:RT.typing g a (pack_ln (Tv_Type u)))
-  (p_typing:RT.typing g p vprop_tm)
-  (q_typing:RT.typing g q (mk_arrow (a, Q_Explicit) vprop_tm))
-
-  : GTot (RT.typing g
-                    (mk_stt_ghost_admit u a p q)
-                    (mk_stt_ghost_comp u a emp_inames_tm p q))
+  (#t:st_term)
+  (#c:comp)
+  (d:st_typing f g t c{T_Admit? d})
+  : GTot (RT.typing (extend_env_l f g)
+                    (elab_st_typing d)
+                    (elab_comp c))
