pulse/examples/dsls/mini_steel/Pulse.Soundness.While.fsti
@@ -1,37 +1,20 @@
 module Pulse.Soundness.While
 
-open FStar.Reflection
-open Pulse.Reflection.Util
+open Pulse.Syntax
+open Pulse.Typing
+open Pulse.Elaborate.Pure
+open Pulse.Elaborate.Core
+open Pulse.Soundness.Common
 
 module RT = Refl.Typing
 
-(*
-
- g |- inv  : bool -> vprop
- g |- cond : stt<0> bool (exists_ inv) inv
- g |- body : stt<0> unit (inv true) (fun _ -> exists_ inv)
- -------------------------------------------------------------------------
- g |- while inv cond body : stt<0> unit (exists_ inv) (fun _ -> inv false)
-
-*)
-
 val while_soundness
+  (#f:stt_env)
   (#g:env)
-  (#inv:term)
-  (#cond:term)
-  (#body:term)
-  (inv_typing:RT.typing g
-                     inv
-                     (mk_arrow (bool_tm, Q_Explicit) vprop_tm))
-  (cond_typing:RT.typing g
-                      cond
-                      (mk_stt_comp uzero bool_tm (mk_exists uzero bool_tm inv) inv))
-  (body_typing:RT.typing g
-                      body
-                      (mk_stt_comp uzero unit_tm
-                         (pack_ln (Tv_App inv (true_tm, Q_Explicit)))
-                         (mk_abs unit_tm Q_Explicit (mk_exists uzero bool_tm inv))))
-  : RT.typing g
-           (mk_while inv cond body)
-           (mk_stt_comp uzero unit_tm (mk_exists uzero bool_tm inv)
-              (mk_abs unit_tm Q_Explicit (pack_ln (Tv_App inv (false_tm, Q_Explicit)))))
+  (#t:st_term)
+  (#c:comp)
+  (d:st_typing f g t c{T_While? d})
+  (soundness: soundness_t d)
+  : GTot (RT.typing (extend_env_l f g)
+                    (elab_st_typing d)
+                    (elab_comp c))
