pulse/examples/dsls/mini_steel/Pulse.Steel.Wrapper.Typing.fst
@@ -1,0 +1,26 @@
+module Pulse.Steel.Wrapper.Typing
+
+open FStar.Reflection
+open Pulse.Reflection.Util
+
+module RT = Refl.Typing
+
+let return_stt_typing _ _ _ = admit ()
+let return_stt_noeq_typing _ _ _ = admit ()
+let return_stt_atomic_typing _ _ _ = admit ()
+let return_stt_atomic_noeq_typing _ _ _ = admit ()
+let return_stt_ghost_typing _ _ _ = admit ()
+let return_stt_ghost_noeq_typing _ _ _ = admit ()
+
+let while_typing _ _ _ = admit ()
+
+let par_typing _ _ _ _ _ _ _ _ _ = admit ()
+
+let exists_inversion _ = admit ()
+let elim_exists_typing _ _ _ = admit ()
+let intro_exists_typing _ _ _ = admit ()
+let intro_exists_erased_typing _ _ _ = admit ()
+
+let stt_admit_typing _ _ _ = admit ()
+let stt_atomic_admit_typing _ _ _ = admit ()
+let stt_ghost_admit_typing _ _ _ = admit ()
