pulse/examples/dsls/mini_steel/Pulse.Steel.Wrapper.Typing.fsti
@@ -1,0 +1,322 @@
+module Pulse.Steel.Wrapper.Typing
+
+open FStar.Reflection
+open Pulse.Reflection.Util
+
+module RT = Refl.Typing
+
+let return_post_with_eq (u:universe) (a:term) (e:term) (p:term) (x:var) : term =
+  let x_tm = RT.var_as_term x in
+  let eq2_tm =
+    let t = pack_ln (Tv_UInst (pack_fv (mk_steel_wrapper_lid "eq2_prop")) [u]) in
+    let t = pack_ln (Tv_App t (a, Q_Implicit)) in
+    let t = pack_ln (Tv_App t (x_tm, Q_Explicit)) in
+    pack_ln (Tv_App t (e, Q_Explicit)) in
+
+  let p_app_x = pack_ln (Tv_App p (x_tm, Q_Explicit)) in
+  
+  let star_tm = mk_star p_app_x eq2_tm in
+
+  mk_abs a Q_Explicit (RT.open_or_close_term' star_tm (RT.CloseVar x) 0)
+
+val return_stt_typing
+  (#g:env)
+  (#u:universe)
+  (#a:term)
+  (#e:term)
+  (#p:term)
+  (x:var{None? (RT.lookup_bvar g x)})
+  (a_typing:RT.typing g a (pack_ln (Tv_Type u)))
+  (e_typing:RT.typing g e a)
+  (p_typing:RT.typing g p (mk_arrow (a, Q_Explicit) vprop_tm))
+
+  : GTot (RT.typing g
+                    (mk_stt_return u a e p)
+                    (mk_stt_comp u a
+                       (pack_ln (Tv_App p (e, Q_Explicit)))
+                       (return_post_with_eq u a e p x)))
+
+val return_stt_noeq_typing
+  (#g:env)
+  (#u:universe)
+  (#a:term)
+  (#x:term)
+  (#p:term)
+  (a_typing:RT.typing g a (pack_ln (Tv_Type u)))
+  (x_typing:RT.typing g x a)
+  (p_typing:RT.typing g p (mk_arrow (a, Q_Explicit) vprop_tm))
+
+  : GTot (RT.typing g
+                    (mk_stt_return u a x p)
+                    (mk_stt_comp u a (pack_ln (Tv_App p (x, Q_Explicit))) p))
+
+val return_stt_atomic_typing
+  (#g:env)
+  (#u:universe)
+  (#a:term)
+  (#e:term)
+  (#p:term)
+  (x:var{None? (RT.lookup_bvar g x)})
+  (a_typing:RT.typing g a (pack_ln (Tv_Type u)))
+  (e_typing:RT.typing g e a)
+  (p_typing:RT.typing g p (mk_arrow (a, Q_Explicit) vprop_tm))
+
+  : GTot (RT.typing g
+                    (mk_stt_atomic_return u a e p)
+                    (mk_stt_atomic_comp u a emp_inames_tm
+                       (pack_ln (Tv_App p (e, Q_Explicit)))
+                       (return_post_with_eq u a e p x)))
+
+val return_stt_atomic_noeq_typing
+  (#g:env)
+  (#u:universe)
+  (#a:term)
+  (#x:term)
+  (#p:term)
+  (a_typing:RT.typing g a (pack_ln (Tv_Type u)))
+  (x_typing:RT.typing g x a)
+  (p_typing:RT.typing g p (mk_arrow (a, Q_Explicit) vprop_tm))
+
+  : GTot (RT.typing g
+                    (mk_stt_atomic_return_noeq u a x p)
+                    (mk_stt_atomic_comp u a emp_inames_tm (pack_ln (Tv_App p (x, Q_Explicit))) p))
+
+val return_stt_ghost_typing
+  (#g:env)
+  (#u:universe)
+  (#a:term)
+  (#e:term)
+  (#p:term)
+  (x:var{None? (RT.lookup_bvar g x)})
+  (a_typing:RT.typing g a (pack_ln (Tv_Type u)))
+  (e_typing:RT.typing g e a)
+  (p_typing:RT.typing g p (mk_arrow (a, Q_Explicit) vprop_tm))
+
+  : GTot (RT.typing g
+                    (mk_stt_ghost_return u a e p)
+                    (mk_stt_ghost_comp u a emp_inames_tm
+                       (pack_ln (Tv_App p (e, Q_Explicit)))
+                       (return_post_with_eq u a e p x)))
+
+val return_stt_ghost_noeq_typing
+  (#g:env)
+  (#u:universe)
+  (#a:term)
+  (#x:term)
+  (#p:term)
+  (a_typing:RT.typing g a (pack_ln (Tv_Type u)))
+  (x_typing:RT.typing g x a)
+  (p_typing:RT.typing g p (mk_arrow (a, Q_Explicit) vprop_tm))
+
+  : GTot (RT.typing g
+                    (mk_stt_ghost_return_noeq u a x p)
+                    (mk_stt_ghost_comp u a emp_inames_tm (pack_ln (Tv_App p (x, Q_Explicit))) p))
+
+(*
+
+ g |- inv  : bool -> vprop
+ g |- cond : stt<0> bool (exists_ inv) inv
+ g |- body : stt<0> unit (inv true) (fun _ -> exists_ inv)
+ -------------------------------------------------------------------------
+ g |- while inv cond body : stt<0> unit (exists_ inv) (fun _ -> inv false)
+
+*)
+
+val while_typing
+  (#g:env)
+  (#inv:term)
+  (#cond:term)
+  (#body:term)
+  (inv_typing:RT.typing g
+                     inv
+                     (mk_arrow (bool_tm, Q_Explicit) vprop_tm))
+  (cond_typing:RT.typing g
+                      cond
+                      (mk_stt_comp uzero bool_tm (mk_exists uzero bool_tm inv) inv))
+  (body_typing:RT.typing g
+                      body
+                      (mk_stt_comp uzero unit_tm
+                         (pack_ln (Tv_App inv (true_tm, Q_Explicit)))
+                         (mk_abs unit_tm Q_Explicit (mk_exists uzero bool_tm inv))))
+  : RT.typing g
+           (mk_while inv cond body)
+           (mk_stt_comp uzero unit_tm (mk_exists uzero bool_tm inv)
+              (mk_abs unit_tm Q_Explicit (pack_ln (Tv_App inv (false_tm, Q_Explicit)))))
+
+let par_post (u:universe) (aL aR:term) (postL postR:term) (x:var) : term =
+  let x_tm = RT.var_as_term x in
+  let postL = pack_ln (Tv_App postL (mk_fst u u aL aR x_tm, Q_Explicit)) in
+  let postR = pack_ln (Tv_App postR (mk_snd u u aL aR x_tm, Q_Explicit)) in
+  let post = mk_star postL postR in
+  RT.open_or_close_term' post (RT.CloseVar x) 0
+
+val par_typing
+  (#g:env)
+  (#u:universe)
+  (#aL #aR:term)
+  (#preL #postL:term)
+  (#preR #postR:term)
+  (#eL #eR:term)
+  (x:var{None? (RT.lookup_bvar g x)})
+  (aL_typing:RT.typing g aL (pack_ln (Tv_Type u)))
+  (aR_typing:RT.typing g aR (pack_ln (Tv_Type u)))
+  (preL_typing:RT.typing g preL vprop_tm)
+  (postL_typing:RT.typing g postL (mk_arrow (aL, Q_Explicit) vprop_tm))
+  (preR_typing:RT.typing g preR vprop_tm)
+  (postR_typing:RT.typing g postR (mk_arrow (aR, Q_Explicit) vprop_tm))
+  (eL_typing:RT.typing g eL (mk_stt_comp u aL preL postL))
+  (eR_typing:RT.typing g eR (mk_stt_comp u aR preR postR))
+
+  : GTot (RT.typing g
+                    (mk_par u aL aR preL postL preR postR eL eR)
+                    (mk_stt_comp u (mk_tuple2 u u aL aR)
+                       (mk_star preL preR)
+                       (mk_abs (mk_tuple2 u u aL aR) Q_Explicit (par_post u aL aR postL postR x))))
+
+val exists_inversion
+  (#g:env)
+  (#u:universe)
+  (#a:term)
+  (#p:term)
+  (e_typing:RT.typing g
+                      (mk_exists u a p)
+                      vprop_tm)
+  : GTot (RT.typing g
+                    p
+                   (mk_arrow (a, Q_Explicit) vprop_tm))
+
+(*
+
+ g |- a : Type u
+ g |- p : a -> vprop
+ ----------------------------------------------------------------
+ g |- elim_exists<u> #a p : stt_ghost<u> a empty (exists_<u> p) (fun x -> p (reveal x))
+
+*)
+
+let elim_exists_post_body (u:universe) (a:term) (p:term) (x:var) =
+  let x_tm = RT.var_as_term x in
+  let reveal_x = mk_reveal u a x_tm in
+  let post = pack_ln (Tv_App p (reveal_x, Q_Explicit)) in
+  RT.open_or_close_term' post (RT.CloseVar x) 0
+
+let elim_exists_post (u:universe) (a:term) (p:term) (x:var) =
+  let erased_a = mk_erased u a in
+  mk_abs erased_a Q_Explicit (elim_exists_post_body u a p x)
+
+val elim_exists_typing
+  (#g:env)
+  (#u:universe)
+  (#a:term)
+  (#p:term)
+  (x:var{None? (RT.lookup_bvar g x)})
+  (a_typing:RT.typing g a (pack_ln (Tv_Type u)))
+  (p_typing:RT.typing g p (mk_arrow (a, Q_Explicit) vprop_tm))
+  : GTot (RT.typing g
+                 (mk_elim_exists u a p)
+                 (mk_stt_ghost_comp
+                    u
+                    (mk_erased u a) 
+                    emp_inames_tm
+                    (mk_exists u a p)
+                    (elim_exists_post u a p x)))
+
+(*
+
+ g |- a : Type u
+ g |- p : a -> vprop
+ g |- e : vprop
+ -------------------------------------------------------------------------
+ g |- intro_exists<u> #a p e : stt_ghost<0> unit empty (p e) (fun _ -> exists_ p)
+
+*)
+val intro_exists_typing
+  (#g:env)
+  (#u:universe)
+  (#a:term)
+  (#p:term)
+  (#e:term)
+  (a_typing:RT.typing g a (pack_ln (Tv_Type u)))
+  (p_typing:RT.typing g p (mk_arrow (a, Q_Explicit) vprop_tm))
+  (e_typing:RT.typing g e a)
+  : GTot (RT.typing g
+                 (mk_intro_exists u a p e)
+                 (mk_stt_ghost_comp uzero unit_tm emp_inames_tm
+                    (pack_ln (Tv_App p (e, Q_Explicit)))
+                    (mk_abs unit_tm Q_Explicit (mk_exists u a p))))
+
+(*
+
+ g |- a : Type u
+ g |- p : a -> vprop
+ g |- e : vprop
+ -------------------------------------------------------------------------
+ g |- intro_exists<u> #a p e : stt_ghost<0> unit empty (p e) (fun _ -> exists_ p)
+
+*)
+val intro_exists_erased_typing
+  (#g:env)
+  (#u:universe)
+  (#a:term)
+  (#p:term)
+  (#e:term)
+  (a_typing:RT.typing g a (pack_ln (Tv_Type u)))
+  (p_typing:RT.typing g p (mk_arrow (a, Q_Explicit) vprop_tm))
+  (e_typing:RT.typing g e (mk_erased u a))
+  : GTot (RT.typing g
+                 (mk_intro_exists_erased u a p e)
+                 (mk_stt_ghost_comp uzero unit_tm emp_inames_tm
+                    (pack_ln (Tv_App p (mk_reveal u a e, Q_Explicit)))
+                    (mk_abs unit_tm Q_Explicit (mk_exists u a p))))
+
+(*
+
+ g |- a : Type u
+ g |- p : vprop
+ g |- q : a -> vprop
+ ------------------------------------------
+ g |- stt_admit a p q : stt a p q
+
+*)
+
+val stt_admit_typing
+  (#g:env)
+  (#u:universe)
+  (#a:term)
+  (#p:term)
+  (#q:term)
+  (a_typing:RT.typing g a (pack_ln (Tv_Type u)))
+  (p_typing:RT.typing g p vprop_tm)
+  (q_typing:RT.typing g q (mk_arrow (a, Q_Explicit) vprop_tm))
+
+  : GTot (RT.typing g
+                    (mk_stt_admit u a p q)
+                    (mk_stt_comp u a p q))
+               
+val stt_atomic_admit_typing
+  (#g:env)
+  (#u:universe)
+  (#a:term)
+  (#p:term)
+  (#q:term)
+  (a_typing:RT.typing g a (pack_ln (Tv_Type u)))
+  (p_typing:RT.typing g p vprop_tm)
+  (q_typing:RT.typing g q (mk_arrow (a, Q_Explicit) vprop_tm))
+
+  : GTot (RT.typing g
+                    (mk_stt_atomic_admit u a p q)
+                    (mk_stt_atomic_comp u a emp_inames_tm p q))
+
+val stt_ghost_admit_typing
+  (#g:env)
+  (#u:universe)
+  (#a:term)
+  (#p:term)
+  (#q:term)
+  (a_typing:RT.typing g a (pack_ln (Tv_Type u)))
+  (p_typing:RT.typing g p vprop_tm)
+  (q_typing:RT.typing g q (mk_arrow (a, Q_Explicit) vprop_tm))
+
+  : GTot (RT.typing g
+                    (mk_stt_ghost_admit u a p q)
+                    (mk_stt_ghost_comp u a emp_inames_tm p q))
